tests/lean/1062.lean
@@ -1,11 +1,11 @@
 example : if x = 0 then y + x = y else x ≠ 0 := by
-  simp (config := { contextual := true })
+  simp (config := { contextual := true, decide := true })
 
 example : if x = 0 then y + x = y else x ≠ 0 := by
   split
   simp_all
-  simp_all
+  simp_all (config := { decide := true })
 
 example : if x = 0 then y + x = y else x ≠ 0 := by
-  simp (config := { contextual := true })
+  simp (config := { contextual := true, decide := true })
   split -- Error: no goals to be solved
