tests/lean/run/1194.lean
@@ -1,6 +1,6 @@
 variable {f: Fin l} {f₀: Fin 0} (h: l = 0) (h': (h▸f) = f₀)
 example: l = 0              := by simp_all
-example (h'': l ≠ 0): False := by simp_all
+example (h'': l ≠ 0): False := by simp_all (config := { decide := true })
 
-example: l = 0              := by simp[*] at *
-example (h'': l ≠ 0): False := by simp[*] at *
+example: l = 0              := by simp [*] at *
+example (h'': l ≠ 0): False := by simp (config := { decide := true }) [*] at *
