tests/lean/run/simpLoopBug.lean
@@ -1,1 +1,1 @@
-example (a : α) : ¬ some (some a) = some none := by simp
+example (a : α) : ¬ some (some a) = some none := by simp (config := { decide := true })
