tests/lean/run/toArrayEq.lean
@@ -3,10 +3,10 @@ inductive Foo
   | foos : Array Foo → Foo
   deriving BEq
 
-example : Foo.foo 0 ≠ Foo.foo 1 := by simp
+example : Foo.foo 0 ≠ Foo.foo 1 := by simp (config := { decide := true })
 
-example : #[0] ≠ #[1] := by simp
+example : #[0] ≠ #[1] := by simp (config := { decide := true })
 
-example : #[Foo.foo 0] ≠ #[Foo.foo 1] := by simp
+example : #[Foo.foo 0] ≠ #[Foo.foo 1] := by simp (config := { decide := true })
 
-example : Foo.foos #[.foo 0] ≠ Foo.foos #[.foo 1] := by simp
+example : Foo.foos #[.foo 0] ≠ Foo.foos #[.foo 1] := by simp (config := { decide := true })
