tests/lean/unfold1.lean
@@ -11,7 +11,7 @@ decreasing_by apply Nat.lt_succ_self
 
 theorem isEven_double (x : Nat) : isEven (2 * x) = true := by
   induction x with
-  | zero => simp
+  | zero => simp (config := { decide := true })
   | succ x ih =>
     unfold isEven
     trace_state
